$$
\begin{aligned*}
{} - AC(D,B) + A(C,B)D - C(D,A)B + (C,A)DB & = & {} - \cancel{ACDB} - \cancel{ACBD} \\
                                           &   & {} + \cancel{ACBD} + ABCD          \\
                                           &   & {} - CDAB          - \cancel{CADB} \\
                                           &   & {} + \cancel{CADB} + \cancel{ACDB} \\\\\\
                                           & = & {} ABCD            - CDAB
\end{aligned*}
$$

$$
\begin{align*}
{} - AC(D,B) + A(C,B)D - C(D,A)B + (C,A)DB &= {} - \cancel{ACDB} - \cancel{ACBD} \\\\
                                           & \mathrel{\phantom{=}} {} + \cancel{ACBD} + ABCD \\\\
                                           & \mathrel{\phantom{=}} {} - CDAB - \cancel{CADB} \\\\
                                           & \mathrel{\phantom{=}} {} + \cancel{CADB} + \cancel{ACDB} \\\\\\
                                           & = ABCD - CDAB
\end{align*}
$$

$$
\begin{align*}
{} - AC(D,B) + A(C,B)D - C(D,A)B + (C,A)DB & = {} - \cancel{ACDB} - \cancel{ACBD} \\\\
                                           &   {} + \cancel{ACBD} + ABCD \\\\
                                           &   {} - CDAB - \cancel{CADB} \\\\
                                           &   {} + \cancel{CADB} + \cancel{ACDB} \\\\\\
                                           & = ABCD - CDAB
\end{align*}
$$


$$
\begin{alignat}{5}
    A & =       & B                                     \\
      &         & B & =     & C                         \\
      &         &   &       & C & =     & D             \\
      & ABCDEFG &   &       &   &       & D & = & E 
\end{alignat}
$$

$$
\begin{alignat}{5}
{} - AC(D,B) + A(C,B)D - C(D,A)B + (C,A)DB &= & {} - \cancel{ACDB} - \cancel{ACBD} \\
                                           &  & {} + \cancel{ACBD} + ABCD          \\
                                           &  & {} - CDAB          - \cancel{CADB} \\
                                           &  & {} + \cancel{CADB} + \cancel{ACDB} \\\\\\
                                           &= & ABCD - CDAB
\end{alignat}
$$
